\documentclass[margin=0.1cm,varwidth=500cm]{standalone}
\usepackage{ebproof}
\usepackage{amssymb}

\begin{document}
\begin{prooftree}
\infer0[$(Ax)$]{\rightarrow,\land,\land,\neg \vdash \neg}
\infer1[$(\neg\vdash)$]{ \neg \neg,\rightarrow,\land,\land,\neg \vdash }
\infer1[$(\vdash\neg)$]{\rightarrow,\land,\land,\neg \vdash  \neg ( \neg \neg)}
\infer0[$(Ax)$]{\rightarrow,\land,\land,\neg \vdash \neg}
\infer1[$(\neg\vdash)$]{ \neg \neg,\rightarrow,\land,\land,\neg \vdash }
\infer1[$(\vdash\neg)$]{\rightarrow,\land,\land,\neg \vdash  \neg ( \neg \neg)}
\infer1[$(\vdash\neg)$]{\land,\land,\neg \vdash  \neg \rightarrow, \neg ( \neg \neg)}
\infer2[$(\rightarrow\vdash)$]{( \neg \rightarrow) \rightarrow \rightarrow,\land,\land,\neg \vdash  \neg ( \neg \neg)}
\infer1[$(\vdash\rightarrow)$]{\land,\land,\neg \vdash (( \neg \rightarrow) \rightarrow \rightarrow) \rightarrow ( \neg ( \neg \neg))}
\infer1[$(\land\vdash)$]{\land \land \land,\neg \vdash (( \neg \rightarrow) \rightarrow \rightarrow) \rightarrow ( \neg ( \neg \neg))}
\infer0[$(Ax)$]{\rightarrow,\neg \vdash  \neg ( \neg \neg),\rightarrow,\rightarrow}
\infer0[$(Ax)$]{\rightarrow,\neg \vdash  \neg ( \neg \neg),\rightarrow,\rightarrow}
\infer1[$(\vdash\neg)$]{\neg \vdash  \neg \rightarrow, \neg ( \neg \neg),\rightarrow,\rightarrow}
\infer2[$(\rightarrow\vdash)$]{( \neg \rightarrow) \rightarrow \rightarrow,\neg \vdash  \neg ( \neg \neg),\rightarrow,\rightarrow}
\infer1[$(\vdash\rightarrow)$]{\neg \vdash (( \neg \rightarrow) \rightarrow \rightarrow) \rightarrow ( \neg ( \neg \neg)),\rightarrow,\rightarrow}
\infer1[$(\neg\vdash)$]{ \neg \rightarrow,\neg \vdash \rightarrow,(( \neg \rightarrow) \rightarrow \rightarrow) \rightarrow ( \neg ( \neg \neg))}
\infer1[$(\vdash\rightarrow)$]{\neg \vdash ( \neg \rightarrow) \rightarrow \rightarrow,(( \neg \rightarrow) \rightarrow \rightarrow) \rightarrow ( \neg ( \neg \neg))}
\infer2[$(\rightarrow\vdash)$]{(( \neg \rightarrow) \rightarrow \rightarrow) \rightarrow (\land \land \land),\neg \vdash (( \neg \rightarrow) \rightarrow \rightarrow) \rightarrow ( \neg ( \neg \neg))}
\infer1[$(\vdash\rightarrow)$]{\neg \vdash ((( \neg \rightarrow) \rightarrow \rightarrow) \rightarrow (\land \land \land)) \rightarrow ((( \neg \rightarrow) \rightarrow \rightarrow) \rightarrow ( \neg ( \neg \neg)))}
\infer1[$(\vdash\neg)$]{ \vdash  \neg \neg,((( \neg \rightarrow) \rightarrow \rightarrow) \rightarrow (\land \land \land)) \rightarrow ((( \neg \rightarrow) \rightarrow \rightarrow) \rightarrow ( \neg ( \neg \neg)))}
\infer1[$(\neg\vdash)$]{ \neg ( \neg \neg) \vdash ((( \neg \rightarrow) \rightarrow \rightarrow) \rightarrow (\land \land \land)) \rightarrow ((( \neg \rightarrow) \rightarrow \rightarrow) \rightarrow ( \neg ( \neg \neg)))}
\infer0[$(Ax)$]{\land,\land \vdash (( \neg \rightarrow) \rightarrow \rightarrow) \rightarrow ( \neg ( \neg \neg)),\lor,\lor,\land}
\infer1[$(\land\vdash)$]{\land \land \land \vdash (( \neg \rightarrow) \rightarrow \rightarrow) \rightarrow ( \neg ( \neg \neg)),\lor,\lor,\land}
\infer0[$(Ax)$]{\rightarrow \vdash  \neg ( \neg \neg),\rightarrow,\rightarrow,\lor,\lor,\land}
\infer0[$(Ax)$]{\rightarrow \vdash  \neg ( \neg \neg),\rightarrow,\rightarrow,\lor,\lor,\land}
\infer1[$(\vdash\neg)$]{ \vdash  \neg \rightarrow, \neg ( \neg \neg),\rightarrow,\rightarrow,\lor,\lor,\land}
\infer2[$(\rightarrow\vdash)$]{( \neg \rightarrow) \rightarrow \rightarrow \vdash  \neg ( \neg \neg),\rightarrow,\rightarrow,\lor,\lor,\land}
\infer1[$(\vdash\rightarrow)$]{ \vdash (( \neg \rightarrow) \rightarrow \rightarrow) \rightarrow ( \neg ( \neg \neg)),\rightarrow,\rightarrow,\lor,\lor,\land}
\infer1[$(\neg\vdash)$]{ \neg \rightarrow \vdash \rightarrow,(( \neg \rightarrow) \rightarrow \rightarrow) \rightarrow ( \neg ( \neg \neg)),\lor,\lor,\land}
\infer1[$(\vdash\rightarrow)$]{ \vdash ( \neg \rightarrow) \rightarrow \rightarrow,(( \neg \rightarrow) \rightarrow \rightarrow) \rightarrow ( \neg ( \neg \neg)),\lor,\lor,\land}
\infer2[$(\rightarrow\vdash)$]{(( \neg \rightarrow) \rightarrow \rightarrow) \rightarrow (\land \land \land) \vdash (( \neg \rightarrow) \rightarrow \rightarrow) \rightarrow ( \neg ( \neg \neg)),\lor,\lor,\land}
\infer1[$(\vdash\rightarrow)$]{ \vdash ((( \neg \rightarrow) \rightarrow \rightarrow) \rightarrow (\land \land \land)) \rightarrow ((( \neg \rightarrow) \rightarrow \rightarrow) \rightarrow ( \neg ( \neg \neg))),\lor,\lor,\land}
\infer1[$(\vdash\lor)$]{ \vdash \lor \lor \lor,((( \neg \rightarrow) \rightarrow \rightarrow) \rightarrow (\land \land \land)) \rightarrow ((( \neg \rightarrow) \rightarrow \rightarrow) \rightarrow ( \neg ( \neg \neg))),\land}
\infer0[$(Ax)$]{\land,\land \vdash (( \neg \rightarrow) \rightarrow \rightarrow) \rightarrow ( \neg ( \neg \neg)),\lor,\lor,\land}
\infer1[$(\land\vdash)$]{\land \land \land \vdash (( \neg \rightarrow) \rightarrow \rightarrow) \rightarrow ( \neg ( \neg \neg)),\lor,\lor,\land}
\infer0[$(Ax)$]{\rightarrow \vdash  \neg ( \neg \neg),\rightarrow,\rightarrow,\lor,\lor,\land}
\infer0[$(Ax)$]{\rightarrow \vdash  \neg ( \neg \neg),\rightarrow,\rightarrow,\lor,\lor,\land}
\infer1[$(\vdash\neg)$]{ \vdash  \neg \rightarrow, \neg ( \neg \neg),\rightarrow,\rightarrow,\lor,\lor,\land}
\infer2[$(\rightarrow\vdash)$]{( \neg \rightarrow) \rightarrow \rightarrow \vdash  \neg ( \neg \neg),\rightarrow,\rightarrow,\lor,\lor,\land}
\infer1[$(\vdash\rightarrow)$]{ \vdash (( \neg \rightarrow) \rightarrow \rightarrow) \rightarrow ( \neg ( \neg \neg)),\rightarrow,\rightarrow,\lor,\lor,\land}
\infer1[$(\neg\vdash)$]{ \neg \rightarrow \vdash \rightarrow,(( \neg \rightarrow) \rightarrow \rightarrow) \rightarrow ( \neg ( \neg \neg)),\lor,\lor,\land}
\infer1[$(\vdash\rightarrow)$]{ \vdash ( \neg \rightarrow) \rightarrow \rightarrow,(( \neg \rightarrow) \rightarrow \rightarrow) \rightarrow ( \neg ( \neg \neg)),\lor,\lor,\land}
\infer2[$(\rightarrow\vdash)$]{(( \neg \rightarrow) \rightarrow \rightarrow) \rightarrow (\land \land \land) \vdash (( \neg \rightarrow) \rightarrow \rightarrow) \rightarrow ( \neg ( \neg \neg)),\lor,\lor,\land}
\infer1[$(\vdash\rightarrow)$]{ \vdash ((( \neg \rightarrow) \rightarrow \rightarrow) \rightarrow (\land \land \land)) \rightarrow ((( \neg \rightarrow) \rightarrow \rightarrow) \rightarrow ( \neg ( \neg \neg))),\lor,\lor,\land}
\infer1[$(\vdash\lor)$]{ \vdash \lor \lor \lor,((( \neg \rightarrow) \rightarrow \rightarrow) \rightarrow (\land \land \land)) \rightarrow ((( \neg \rightarrow) \rightarrow \rightarrow) \rightarrow ( \neg ( \neg \neg))),\land}
\infer2[$(\vdash\land)$]{ \vdash \land \land \land,\lor \lor \lor,((( \neg \rightarrow) \rightarrow \rightarrow) \rightarrow (\land \land \land)) \rightarrow ((( \neg \rightarrow) \rightarrow \rightarrow) \rightarrow ( \neg ( \neg \neg)))}
\infer1[$(\vdash\lor)$]{ \vdash (\land \land \land) \lor \lor \lor \lor,((( \neg \rightarrow) \rightarrow \rightarrow) \rightarrow (\land \land \land)) \rightarrow ((( \neg \rightarrow) \rightarrow \rightarrow) \rightarrow ( \neg ( \neg \neg)))}
\infer2[$(\rightarrow\vdash)$]{((\land \land \land) \lor \lor \lor \lor) \rightarrow ( \neg ( \neg \neg)) \vdash ((( \neg \rightarrow) \rightarrow \rightarrow) \rightarrow (\land \land \land)) \rightarrow ((( \neg \rightarrow) \rightarrow \rightarrow) \rightarrow ( \neg ( \neg \neg)))}
\infer1[$(\vdash\rightarrow)$]{ \vdash (((\land \land \land) \lor \lor \lor \lor) \rightarrow ( \neg ( \neg \neg))) \rightarrow (((( \neg \rightarrow) \rightarrow \rightarrow) \rightarrow (\land \land \land)) \rightarrow ((( \neg \rightarrow) \rightarrow \rightarrow) \rightarrow ( \neg ( \neg \neg))))}
\end{prooftree}


Valid ? true

\end{document}
